src/Spec/Protocol.v
@@ -18,16 +18,17 @@ Section Protocol.
   Variable op_allow : OpProtocol.
 
   Definition nilpotent_step : OpSemantics opT State :=
-    fun T op tid s r s' =>
+    fun T op tid s r s' evs =>
       ( op_allow op tid s /\
-        lo_step op tid s r s' ) \/
+        lo_step op tid s r s' evs ) \/
       ( ~ op_allow op tid s /\
-        s' = s ).
+        s' = s /\
+        evs = nil ).
 
   Definition restricted_step : OpSemantics opT State :=
-    fun T op tid s r s' =>
+    fun T op tid s r s' evs =>
       op_allow op tid s /\
-      lo_step op tid s r s'.
+      lo_step op tid s r s' evs.
 
   Variable loopInv : forall (s : State) (tid : nat), Prop.
 
@@ -55,9 +56,6 @@ Section Protocol.
       exec_any restricted_step tid s' (p v') r s'' ->
       loopInv s'' tid) ->
     follows_protocol_proc tid s (Until c p v)
-  | FollowsProtocolProcLog :
-    forall T (v : T),
-    follows_protocol_proc tid s (Log v)
   | FollowsProtocolProcRet :
     forall T (v : T),
     follows_protocol_proc tid s (Ret v)
@@ -71,17 +69,17 @@ Section Protocol.
 
 
   Variable allowed_stable :
-    forall `(op : opT T) `(op' : opT T') tid tid' s s' r,
+    forall `(op : opT T) `(op' : opT T') tid tid' s s' r evs,
       tid <> tid' ->
       op_allow op tid s ->
-      restricted_step op' tid' s r s' ->
+      restricted_step op' tid' s r s' evs ->
       op_allow op tid s'.
 
   Variable loopInv_stable :
-    forall `(op' : opT T') tid tid' s s' r,
+    forall `(op' : opT T') tid tid' s s' r evs,
       tid <> tid' ->
       loopInv s tid ->
-      restricted_step op' tid' s r s' ->
+      restricted_step op' tid' s r s' evs ->
       loopInv s' tid.
 
   Theorem follows_protocol_preserves_exec_tid' :
@@ -170,10 +168,10 @@ Section Protocol.
   Qed.
 
   Theorem follows_protocol_stable :
-    forall `(p : proc opT T) `(op' : opT T') tid tid' s s' r,
+    forall `(p : proc opT T) `(op' : opT T') tid tid' s s' r evs,
       tid <> tid' ->
       follows_protocol_proc tid s p ->
-      restricted_step op' tid' s r s' ->
+      restricted_step op' tid' s r s' evs ->
       follows_protocol_proc tid s' p.
   Proof.
     intros.
